backend/Linearizeproof.v
@@ -710,7 +710,7 @@ Lemma transf_initial_states:
 Proof.
   intros. inversion H.
   exploit function_ptr_translated; eauto. intros [tf [A B]].
-  exists (Callstate nil tf (Locmap.init Vundef) m0); split.
+  exists (Callstate nil tf Locmap.init m0); split.
   econstructor; eauto. eapply (Genv.init_mem_transf_partial TRANSF); eauto.
   rewrite (match_program_main TRANSF).
   rewrite symbols_preserved. eauto.
