backend/Registerfile.v
@@ -1,0 +1,184 @@
+(* *********************************************************************)
+(*                                                                     *)
+(*              The Compcert verified compiler                         *)
+(*                                                                     *)
+(*          Gergö Barany, INRIA Paris-Rocquencourt                     *)
+(*                                                                     *)
+(*  Copyright Institut National de Recherche en Informatique et en     *)
+(*  Automatique.  All rights reserved.  This file is distributed       *)
+(*  under the terms of the INRIA Non-Commercial License Agreement.     *)
+(*                                                                     *)
+(* *********************************************************************)
+
+Require Import OrderedType.
+Require Import Coqlib.
+Require Import Maps.
+Require Import Ordered.
+Require Import AST.
+Require Import Values.
+Require Import Memdata.
+Require Import Memory.
+Require Export Machregs.
+
+Open Scope Z_scope.
+
+(** * Representation of the register file *)
+
+(** The [Regfile] module defines mappings from registers to values. The register
+  file is represented as a kind of memory block containing bytes addressed using
+  register numbers.
+  The register numbers are taken from [IndexedMreg], interpreted as words and
+  scaled internally to bytes. The indices of adjacent 64-bit registers must
+  therefore differ by at least 2. *)
+
+Module Regfile.
+
+  Definition t := ZMap.t memval.
+
+  Definition init := ZMap.init Undef.
+
+  (* A register's address: The index of its first byte. *)
+  Definition addr (r: mreg) : Z := Zpos (IndexedMreg.index r) * 4.
+
+  Remark addr_pos: forall r, addr r > 0.
+  Proof.
+    intros. unfold addr. xomega.
+  Qed.
+
+  (* The address one byte past the end of register [r]. The next nonoverlapping
+     register may start here. *)
+  Definition next_addr (r: mreg) : Z := addr r + AST.typesize (mreg_type r).
+
+  Lemma outside_interval_diff:
+    forall r s, next_addr r <= addr s \/ next_addr s <= addr r -> r <> s.
+  Proof.
+    intros. destruct H; unfold next_addr in H.
+    generalize (AST.typesize_pos (mreg_type r)); intros. contradict H. subst. omega.
+    generalize (AST.typesize_pos (mreg_type s)); intros. contradict H. subst. omega.
+  Qed.
+
+  Lemma address_lt:
+    forall r s,
+    r <> s ->
+    addr r < addr s ->
+    next_addr r <= addr s.
+  Proof.
+    intros. unfold addr in H0.
+    apply IndexedMreg.scaled_index_with_size; omega.
+  Qed.
+
+  Lemma diff_outside_interval:
+    forall r s, r <> s -> next_addr r <= addr s \/ next_addr s <= addr r.
+  Proof.
+    intros.
+    assert (Neq: addr r <> addr s).
+    { unfold addr. contradict H. apply IndexedMreg.index_inj. xomega. }
+    assert (Cases: addr r < addr s \/ addr s < addr r) by omega.
+    destruct Cases.
+    - left. apply address_lt; auto.
+    - right. apply address_lt; auto.
+  Qed.
+
+  Definition chunk_of_mreg (r: mreg) : memory_chunk :=
+    chunk_of_type (mreg_type r).
+
+  Lemma chunk_length:
+    forall r v,
+    Z.to_nat (AST.typesize (mreg_type r)) = length (encode_val (chunk_of_mreg r) v).
+  Proof.
+    intros. rewrite encode_val_length.
+    unfold chunk_of_mreg. destruct (mreg_type r); auto.
+  Qed.
+
+  Definition get_bytes (r: mreg) (rf: t) : list memval :=
+    Mem.getN (Z.to_nat (AST.typesize (mreg_type r))) (addr r) rf.
+
+  Definition get (r: mreg) (rf: t) : val :=
+    decode_val (chunk_of_mreg r) (get_bytes r rf).
+
+  Definition set_bytes (r: mreg) (bytes: list memval) (rf: t) : t :=
+    Mem.setN bytes (addr r) rf.
+
+  Definition set (r: mreg) (v: val) (rf: t) : t :=
+    set_bytes r (encode_val (chunk_of_mreg r) v) rf.
+
+  (* Update the [old] register file by choosing the values for the registers in
+     [rs] from [new]. *)
+  Fixpoint override (rs: list mreg) (new old: t) : t :=
+    match rs with
+    | nil => old
+    | r :: rs' => set r (get r new) (override rs' new old)
+    end.
+
+  Fixpoint undef_regs (rs: list mreg) (rf: t) : t :=
+    match rs with
+    | nil => rf
+    | r :: rs => set r Vundef (undef_regs rs rf)
+    end.
+
+  Lemma gss:
+    forall r v rf,
+    get r (set r v rf) = Val.load_result (chunk_of_mreg r) v.
+  Proof.
+    intros. unfold get, set, get_bytes, set_bytes.
+    erewrite chunk_length. rewrite Mem.getN_setN_same.
+    erewrite <- decode_encode_val_similar; eauto.
+    eapply decode_encode_val_general.
+  Qed.
+
+  Lemma gso:
+    forall r s v rf,
+    r <> s ->
+    get r (set s v rf) = get r rf.
+  Proof.
+    intros. unfold get, set, get_bytes, set_bytes.
+    rewrite Mem.getN_setN_outside; auto.
+    rewrite <- chunk_length.
+    generalize (AST.typesize_pos (mreg_type s)), (AST.typesize_pos (mreg_type r)); intros.
+    apply diff_outside_interval in H. unfold next_addr in H.
+    rewrite !Z2Nat.id; omega.
+  Qed.
+
+  Lemma override_in:
+    forall rs r new old,
+    In r rs -> get r (override rs new old) = get r new.
+  Proof.
+    intros. induction rs; try contradiction.
+    destruct (mreg_eq r a).
+    - subst; simpl; rewrite gss.
+      unfold chunk_of_mreg. rewrite Val.load_result_same; auto.
+      unfold get. rewrite <- type_of_chunk_of_type.
+      apply decode_val_type.
+    - inversion H; try congruence.
+      simpl; rewrite gso; auto.
+  Qed.
+
+  Lemma override_notin:
+    forall r rs new old,
+    ~ In r rs -> get r (override rs new old) = get r old.
+  Proof.
+    intros. induction rs; auto.
+    apply not_in_cons in H. simpl. rewrite gso; intuition auto.
+  Qed.
+
+  Lemma undef_regs_in:
+    forall r rs rf,
+    In r rs -> get r (undef_regs rs rf) = Vundef.
+  Proof.
+    induction rs; simpl; intros. contradiction.
+    destruct (mreg_eq r a).
+    - subst; simpl; rewrite gss.
+      destruct (chunk_of_mreg a); auto.
+    - inversion H; try congruence.
+      simpl; rewrite gso; auto.
+  Qed.
+
+  Lemma undef_regs_notin:
+    forall r rs rf,
+    ~ In r rs -> get r (undef_regs rs rf) = get r rf.
+  Proof.
+    induction rs; auto; intros.
+    apply not_in_cons in H. simpl. rewrite gso; intuition auto.
+  Qed.
+
+End Regfile.
