Makefile
@@ -86,7 +86,7 @@ BACKEND=\
   CSEdomain.v CombineOp.v CSE.v CombineOpproof.v CSEproof.v \
   NeedDomain.v NeedOp.v Deadcode.v Deadcodeproof.v \
   Unusedglob.v Unusedglobproof.v \
-  Machregs.v Locations.v Conventions1.v Conventions.v \
+  Machregs.v Registerfile.v Locations.v Conventions1.v Conventions.v \
   LTL.v LTLtyping.v \
   Allocation.v Allocproof.v \
   Tunneling.v Tunnelingproof.v \
